Wrote rpc lemmas for new crash-safety plan

src/program_proof/lockservice/rpc_durable.v
@@ -13,10 +13,13 @@ Context `{!rpcG Σ R}.
 initialized: Request created and "on its way" to the server.
 done: The reply was computed as is waiting for the client to take notice.
 dead: The client took out ownership of the reply. *)
-Local Definition RPCRequest_durable_inv (γrpc:rpc_names) (γPost:gname) (PreCond : A -> iProp Σ) (PostCond : A -> R -> iProp Σ) (req:RPCRequest) : iProp Σ :=
+Local Definition RPCRequest_durable_inv (γrpc:rpc_names) (γPost γPre:gname) (PreCond : A -> iProp Σ) (PostCond : A -> R -> iProp Σ) (req:RPCRequest) : iProp Σ :=
    "#Hlseq_bound" ∷ req.(CID) fm[[γrpc.(cseq)]]> int.nat req.(Seq)
     ∗ ( (* Initialized, but server has not started processing *)
-      "Hreply" ∷ (req.(CID), req.(Seq)) [[γrpc.(rc)]]↦ None ∗ PreCond req.(Args) ∨ 
+      "Hreply" ∷ (req.(CID), req.(Seq)) [[γrpc.(rc)]]↦ None ∗
+               ((∃ s, req.(CID) fm[[γrpc.(lseq)]]↦{3/4} s) ∨ own γPre (Excl ()) ∗ PreCond req.(Args) ) ∨ 
+      (* Not doing full ownership of the fmcounter becuase we (probably) want to remember the value.
+        Doing 3/4 so we know that if we are given 3/4 ownership, then this disjunction can't be in the first case *)
 
       (* Server has finished processing; two sub-states for wether client has taken PostCond out *)
       req.(CID) fm[[γrpc.(lseq)]]≥ int.nat req.(Seq)
@@ -25,10 +28,46 @@ Local Definition RPCRequest_durable_inv (γrpc:rpc_names) (γPost:gname) (PreCon
       )
     ).
 
-Definition is_durable_RPCRequest (γrpc:rpc_names) (γPost:gname) (PreCond : A -> iProp Σ) (PostCond : A -> R -> iProp Σ) (req:RPCRequest) : iProp Σ :=
-  inv rpcRequestInvN (RPCRequest_durable_inv γrpc γPost PreCond PostCond req).
+Definition is_durable_RPCRequest (γrpc:rpc_names) (γPost γPre:gname) (PreCond : A -> iProp Σ) (PostCond : A -> R -> iProp Σ) (req:RPCRequest) : iProp Σ :=
+  inv rpcRequestInvN (RPCRequest_durable_inv γrpc γPost γPre PreCond PostCond req).
+
+Definition RPCServer_own_processing γrpc (req:@RPCRequest A) lastSeqM lastReplyM : iProp Σ :=
+  (∃ s, req.(CID) fm[[γrpc.(lseq)]]↦{3 / 4} s) -∗
+  RPCServer_own γrpc lastSeqM lastReplyM.
+
+(* TODO: own_processing is actually just a bigSep of ownerships; the -∗ is just a more convenient to use elsewhere*)
+Global Instance RPCServer_own_processing_disc γrpc (req:@RPCRequest A) lastSeqM lastReplyM : Discretizable (RPCServer_own_processing γrpc req lastSeqM lastReplyM).
+Admitted.
+
+
+Lemma server_takes_request (req:@RPCRequest A) γrpc γPost γPre PreCond PostCond lastSeqM lastReplyM (old_seq:u64) :
+  ((map_get lastSeqM req.(CID)).1 = old_seq) →
+  (int.Z req.(Seq) > int.Z old_seq)%Z →
+  is_durable_RPCRequest γrpc γPost γPre PreCond PostCond req -∗
+  RPCServer_own γrpc lastSeqM lastReplyM
+  ={⊤}=∗
+  own γPre (Excl ()) ∗ PreCond req.(Args) ∗
+  RPCServer_own_processing γrpc req lastSeqM lastReplyM.
+Admitted.
+
+Lemma server_executes_durable_request' (req:@RPCRequest A) reply γrpc γPost γPre PreCond PostCond lastSeqM lastReplyM (old_seq:u64) ctx ctx':
+  (* TODO: get rid of this requirement by putting γPre in the postcondition case *)
+  ((map_get lastSeqM req.(CID)).1 = old_seq) →
+  (int.Z req.(Seq) > int.Z old_seq)%Z →
+  is_durable_RPCRequest γrpc γPost γPre PreCond PostCond req -∗
+  is_RPCServer γrpc -∗
+  RPCServer_own_processing γrpc req lastSeqM lastReplyM -∗
+  own γPre (Excl()) -∗
+  (∃ R, R ∗ 
+  (▷ R -∗ ctx ==∗ PostCond req.(Args) reply ∗ ctx')) -∗
+  ctx ={⊤}=∗
+  (RPCReplyReceipt γrpc req reply ∗
+  RPCServer_own γrpc (<[req.(CID):=req.(Seq)]> lastSeqM) (<[req.(CID):=reply]> lastReplyM) ∗
+  ctx').
+Admitted.
 
 (* TODO: allow the fupd under a mask that doesn't contain rpcRequestInvN *)
+(*
 Lemma server_executes_durable_request `{Inhabited R} (req:@RPCRequest A) reply γrpc γPost PreCond PostCond lastSeqM lastReplyM ctx ctx' old_seq :
   ((map_get lastSeqM req.(CID)).1 = old_seq) →
   (int.Z req.(Seq) > int.Z old_seq)%Z →
@@ -134,5 +173,6 @@ Proof.
     lia.
   }
 Qed.
+*)
 
 End rpc_durable.
